Improved swap example

isabelle/Examples/Swap.thy
@@ -1,67 +1,226 @@
 (*<*)
 theory Swap
-  imports Core.Semantics Core.TransactionBound
+  imports Core.Semantics Core.TransactionBound Core.Timeout
 begin
 (*>*)
 
-section \<open>Contract definition\<close>
+section \<open>Simple Swap\<close>
 
-record SwapParty = party           :: Party
-                   currency        :: Token
-                   amount          :: Value
-                   depositDeadline :: Timeout
+text \<open>
+A simple swap contract consists on two parties exchanging some \<^term>\<open>amount\<close> of \<^term>\<open>Token\<close>s 
+atomically. Each participant needs to deposit their tokens into the contract by a certain
+\<^term>\<open>depositDeadline\<close>. If they do, the contract makes the swap and pays the participants, if 
+one of the participant fails to make the deposit, the funds held by the contract can be redeemed 
+by the owner.
+\<close>
+
+subsection \<open>Contract definition\<close>
+
+text \<open>
+To reduce the number of parameters we bundle the information required by each participant into a record.
+\<close>
+
+record SwapParty = 
+  \<comment> \<open>A participant of the contract,\<close>
+  party           :: Party
+  \<comment> \<open>wants to swap an \<^term>\<open>amount\<close> of \<^term>\<open>Token\<close>\<close>
+  amount          :: Value   
+  currency        :: Token    
+  \<comment> \<open>before a deadline\<close>
+  depositDeadline :: Timeout
+
+
+text \<open>The following helper function allows participants to deposit their tokens into the contract. \<close>
 
 fun makeDeposit :: "SwapParty \<Rightarrow> Contract \<Rightarrow> Contract" where 
-  "makeDeposit sp continuation  = 
+  "makeDeposit sp continue  = 
+    \<comment> \<open>The contract waits for a deposit\<close>
     When
-      [ Case (Deposit (party sp) (party sp) (currency sp) (amount sp)) continuation ]
-      (depositDeadline sp)
-      Close  
+      [ 
+        Case 
+          (Deposit 
+            \<comment> \<open>into the internal account of the party\<close>
+            (party sp) 
+            \<comment> \<open>from the party wallet\<close>
+            (party sp) 
+            \<comment> \<open>Amount of tokens\<close>
+            (currency sp) 
+            (amount sp)
+          )
+          \<comment> \<open>Once the deposit has been made, execute the continuation\<close> 
+          continue 
+     ]
+     \<comment> \<open>If the tokens haven't been deposited by the deadline, close the contract.\<close>
+     \<comment> \<open>This will return all current funds to their owners.\<close>
+     (depositDeadline sp) Close  
    "
 
+text \<open>The following helper function makes a \<^term>\<open>Payment\<close> from one party to the other\<close>
 fun makePayment :: "SwapParty \<Rightarrow> SwapParty \<Rightarrow> Contract \<Rightarrow> Contract" where 
-  \<open>makePayment src dest = Pay (party src) (Party (party dest)) (currency src) (amount src)
-  \<close> 
+  "makePayment src dest = 
+    \<comment> \<open>The contract makes a Payment\<close>
+    Pay 
+      \<comment> \<open>from the party internal account\<close>
+      (party src) 
+      \<comment> \<open>to the destination wallet\<close>
+      (Party (party dest)) 
+      \<comment> \<open>of the number of tokens from the source\<close>
+      (currency src) (amount src)
+  " 
 
-fun swap :: \<open>SwapParty \<Rightarrow> SwapParty \<Rightarrow> Contract\<close> where 
-  \<open>swap p1 p2 = makeDeposit p1 
+text \<open>The actual swap contract waits for both parties to make their deposits, then makes the payout
+and closes.\<close>
+fun swap :: "SwapParty \<Rightarrow> SwapParty \<Rightarrow> Contract" where 
+  "swap p1 p2 = makeDeposit p1 
                 ( makeDeposit p2 
                 ( makePayment p1 p2 
                 ( makePayment p2 p1 Close
                 )))
-  \<close>
+  "
 
-section \<open>Swap Example\<close>
+subsection \<open>Example execution\<close>
 
-definition tokenAProvider :: "SwapParty" where
-  \<open>tokenAProvider = 
-     \<lparr> party = Role (BS ''Token A Provider'')
-     , currency = Token (BS ''symbol-a'') (BS ''a'')
-     , amount = Constant 10
-     , depositDeadline = 10
-     \<rparr> \<close> 
+text \<open>Let's define two participants that want to trade USD and ADA in the cardano blockchain.\<close>
 
-definition tokenBProvider  :: "SwapParty" where
-  \<open>tokenBProvider = 
-     \<lparr> party = Role (BS ''Token B Provider'')
-     , currency = Token (BS ''symbol-b'') (BS ''b'')
-     , amount = Constant 20
-     , depositDeadline = 20
-     \<rparr> \<close> 
+definition "adaProvider = Role (BS ''Ada Provider'')"
+definition "dollarProvider = Role (BS ''Dollar Provider'')"
 
-definition "swapExample = swap tokenAProvider tokenBProvider"
+text "In cardano, the ADA symbol is represented by the empty string"
 
-section \<open>Contract guarantees\<close>
+definition "adaToken = Token (BS '''') (BS '''')"
+definition "dollarToken = Token (BS ''85bb65'') (BS ''dollar'')"
 
-proposition maxSwapTransactions: "maxTransactionsInitialState (swap a b) = 2" 
-  by simp
+text \<open>The contract can be created as follow.\<close>
 
+definition
+  "swapExample = 
+    swap 
+      \<comment> \<open>Party A trades 10 lovelaces\<close>
+      \<comment> \<open>deposited before Monday, October 3, 2022 4:00:00 PM GMT\<close>
+      \<lparr> party = adaProvider
+      , amount = Constant 10
+      , currency = adaToken
+      , depositDeadline = 1664812800000
+      \<rparr>
+      \<comment> \<open>Party B trades 20 cents\<close>
+      \<comment> \<open>deposited before Monday, October 3, 2022 5:00:00 PM GMT\<close>
+      \<lparr> party = dollarProvider
+      , amount = Constant 20
+      , currency = dollarToken
+      , depositDeadline = 1664816400000 
+      \<rparr>
+  "
+
+subsubsection \<open>Happy path\<close>
+
+text \<open>If both parties deposit before their deadline,\<close>
+
+definition
+  "happyPathTransactions = 
+    [ 
+      \<comment> \<open>First party deposit\<close>
+      \<lparr> interval = (1664812600000, 1664812700000)
+      , inputs = [
+                  IDeposit 
+                    adaProvider 
+                    adaProvider 
+                    adaToken 
+                    10
+                 ] 
+      \<rparr>
+     \<comment> \<open>Second party deposit\<close>
+    , \<lparr> interval = (1664812900000, 1664813100000)
+      , inputs = [
+                  IDeposit 
+                    dollarProvider
+                    dollarProvider  
+                    dollarToken
+                    20
+                 ]  
+      \<rparr>
+    ]
+  "
+
+text  \<open>payments are made to swap the tokens\<close>
+definition 
+  "happyPathPayments = 
+    [ Payment adaProvider (Party dollarProvider) adaToken 10
+    , Payment dollarProvider (Party adaProvider) dollarToken 20
+    ]
+  "
+
+text \<open>and the contract is closed without emitting a warning\<close>
+
+proposition
+ "playTrace 0 swapExample happyPathTransactions = TransactionOutput txOut
+  \<Longrightarrow> 
+     txOutContract txOut = Close
+     \<and> txOutPayments txOut = happyPathPayments
+     \<and> txOutWarnings txOut = []"
+(*<*)apply (code_simp)
+     apply (auto simp add: happyPathPayments_def  adaProvider_def adaToken_def dollarProvider_def  dollarToken_def)
+     done(*>*)
+
+
+subsection \<open>Contract guarantees\<close>
+
+subsubsection \<open>Number of transactions\<close>
+text \<open>Counting the amount of When's, it is easy to notice that there can be at most two transactions\<close>
+
+proposition (*<*)maxSwapTransactions:(*>*)
+  "maxTransactionsInitialState (swap a b) = 2" 
+(*<*)by simp(*>*)
+
+text \<open>Expressed in a different way, if we use the lemma defined in \secref{sec:transaction-bound} we can
+state that, if the execution of the contract yields a succesful \<^term>\<open>TransactionOutput\<close>, then the number
+of transactions must be lower or equal than @{value "maxTransactionsInitialState (swap a b)"}\<close>
+
+lemma
+  "playTrace 
+      initialTime 
+      (swap a b) 
+      transactions = TransactionOutput txOut
+   \<Longrightarrow> length transactions \<le> 2"
+(*<*)by (metis maxSwapTransactions playTrace_only_accepts_maxTransactionsInitialState)(*>*)
+
+subsubsection \<open>Maximum time\<close>
+
+text \<open>If the deadline of the second party is bigger than the first, then that deadline is the 
+maximum time of the contract.\<close>
+proposition 
+  "sp1 =  \<lparr> party = p1, amount = a1, currency = t1, depositDeadline = d1 \<rparr>   
+   \<Longrightarrow> sp2 = \<lparr> party = p2, amount = a2, currency = t2, depositDeadline = d2 \<rparr>
+   \<Longrightarrow> d2 > d1
+   \<Longrightarrow> d1 > 0
+   \<Longrightarrow> contract = swap sp1 sp2 
+   \<Longrightarrow> maxTimeContract (contract) = d2
+  "
+  (*<*)by simp(*>*)
+
+(*<*)
+\<comment> \<open>Section ommited for the moment\<close>
+text \<open>Expressed in another way, by using the lemma defined in \secref{sec:max-time-guarantee} we can
+guarantee that if we apply an empty transaction after the contract deadline, the contract will close.\<close>
 
 lemma 
-  "playTrace initialTime (swap a b) transactions = TransactionOutput txOut \<Longrightarrow>
-   length transactions \<le> 2"
-  by (metis maxSwapTransactions playTrace_only_accepts_maxTransactionsInitialState)
-
+ "sp1 =  \<lparr> party = p1, amount = a1, currency = t1, depositDeadline = d1 \<rparr>   
+   \<Longrightarrow> sp2 = \<lparr> party = p2, amount = a2, currency = t2, depositDeadline = d2 \<rparr>   
+   \<Longrightarrow> d2 > d1
+   \<Longrightarrow> d1 > 0
+   \<Longrightarrow> contract = swap sp1 sp2 
+   \<Longrightarrow> validAndPositive_state sta
+   \<Longrightarrow> iniTime \<ge> minTime sta
+   \<Longrightarrow> iniTime \<ge> d2
+   \<Longrightarrow> endTime \<ge> iniTime
+   \<Longrightarrow> accounts sta \<noteq> [] \<or> contract \<noteq> Close
+   \<Longrightarrow> isClosedAndEmpty (computeTransaction \<lparr> interval = (iniTime, endTime)
+                                            , inputs = [] \<rparr> sta contract)
+  "
+  using  swapExample_def happyPathTransactions_def dollarProvider_def dollarToken_def adaProvider_def adaToken_def
+  apply (simp_all)
+  oops
+(*>*)
+  
 
 (*<*)
 end
